use bir_symb_transfer function in bir_symbLib for incr, mod2, swap

examples/riscv/common/bir_symbLib.sig
@@ -17,4 +17,8 @@ sig
 
   val bir_symb_analysis : term -> term -> term list -> term -> term -> thm;
 
+  val bir_symb_transfer : term -> term -> term -> term ->
+    thm -> thm -> thm -> thm -> thm ->
+    thm -> thm -> thm -> thm;
+
 end
