examples/riscv/swap/swap_symb_transfScript.sml
@@ -43,13 +43,13 @@ open bir_program_varsTheory;
 
 open distribute_generic_stuffTheory;
 
+open bir_symbLib;
+
 open swapTheory;
 open swap_specTheory;
 open swap_symb_execTheory;
 
 val _ = new_theory "swap_symb_transf";
-
-val birs_state_ss = rewrites (type_rws ``:birs_state_t``);
 
 (* --------------------- *)
 (* Auxiliary definitions *)
@@ -58,331 +58,27 @@ val birs_state_ss = rewrites (type_rws ``:birs_state_t``);
 val init_addr_tm = (snd o dest_eq o concl) swap_init_addr_def;
 val end_addr_tm = (snd o dest_eq o concl) swap_end_addr_def;
 
-val bir_prog_def = bir_swap_prog_def;
-val birenvtyl_def = swap_birenvtyl_def;
-val bspec_pre_def = bspec_swap_pre_def;
-val bspec_post_def = bspec_swap_post_def;
-val prog_vars_def = swap_prog_vars_def;
-
-val symb_analysis_thm = swap_symb_analysis_thm;
-val bsysprecond_thm = swap_bsysprecond_thm;
-val prog_vars_thm = swap_prog_vars_thm;
-
-val bprog_tm = (fst o dest_eq o concl) bir_prog_def;
-val prog_vars_tm = (fst o dest_eq o concl) prog_vars_def;
-
-val birenvtyl_tm = (fst o dest_eq o concl) birenvtyl_def;
-
 val bspec_pre_tm = ``bspec_swap_pre pre_x10 pre_x11 pre_x10_mem_deref pre_x11_mem_deref``;
 val bspec_post_tm = ``bspec_swap_post pre_x10 pre_x11 pre_x10_mem_deref pre_x11_mem_deref``;
-
-val bir_state_init_lbl_tm = (snd o dest_eq o concl o EVAL)
- ``bir_block_pc (BL_Address (Imm64 ^init_addr_tm))``;
-val birs_state_end_lbl_tm = (snd o dest_eq o concl o EVAL)
- ``bir_block_pc (BL_Address (Imm64 ^end_addr_tm))``;
-
-val birs_state_init_pre_tm = ``birs_state_init_pre_GEN
- ^bir_state_init_lbl_tm ^birenvtyl_tm
- (mk_bsysprecond ^bspec_pre_tm ^birenvtyl_tm)``;
-
-val (sys_i, L_s, Pi_f) = (symb_sound_struct_get_sysLPi_fun o concl) symb_analysis_thm;
 
 (* ------------------------------- *)
 (* BIR symbolic execution analysis *)
 (* ------------------------------- *)
 
-Theorem analysis_L_NOTIN_thm[local]:
-  ^birs_state_end_lbl_tm NOTIN ^L_s
-Proof
-  EVAL_TAC
-QED
+val bspec_cont_thm =
+ bir_symb_transfer init_addr_tm end_addr_tm bspec_pre_tm bspec_post_tm
+  bir_swap_prog_def swap_birenvtyl_def bspec_swap_pre_def bspec_swap_post_def swap_prog_vars_def
+  swap_symb_analysis_thm swap_bsysprecond_thm swap_prog_vars_thm;
 
-(* ........................... *)
-(* ........................... *)
-(* ........................... *)
-
-Theorem birs_state_init_pre_EQ_thm[local]:
-  ^((snd o dest_comb) sys_i) = ^birs_state_init_pre_tm
-Proof
-  REWRITE_TAC [birs_state_init_pre_GEN_def, mk_bsysprecond_def, bsysprecond_thm] >>
-  CONV_TAC (computeLib.RESTR_EVAL_CONV [``birs_eval_exp``] THENC birs_stepLib.birs_eval_exp_CONV)
-QED
-
-val analysis_thm =
-  REWRITE_RULE [birs_state_init_pre_EQ_thm, GSYM bir_prog_def] symb_analysis_thm;
-
-Theorem birenvtyl_EVAL_thm[local] =
- (REWRITE_CONV [birenvtyl_def,
-   bir_lifting_machinesTheory.riscv_bmr_vars_EVAL,
-   bir_lifting_machinesTheory.riscv_bmr_temp_vars_EVAL] THENC EVAL)
- birenvtyl_tm;
-
-val birs_state_thm = REWRITE_CONV [birenvtyl_EVAL_thm] birs_state_init_pre_tm;
-
-(* ------ *)
-
-(* now the transfer *)
-
-val birs_symb_symbols_f_sound_prog_thm =
-  (SPEC (inst [Type`:'observation_type` |-> Type.alpha] bprog_tm)
-        bir_symb_soundTheory.birs_symb_symbols_f_sound_thm);
-
-val birs_prop_transfer_thm =
-  (MATCH_MP 
-   symb_prop_transferTheory.symb_prop_transfer_thm
-   birs_symb_symbols_f_sound_prog_thm);
-
-(* ........................... *)
-
-(* P is generic enough *)
-(* taken from "bir_exp_to_wordsLib" *)
-val type_of_bir_exp_thms =
-    let
-      open bir_immTheory
-      open bir_valuesTheory
-      open bir_envTheory
-      open bir_exp_memTheory
-      open bir_bool_expTheory
-      open bir_extra_expsTheory
-      open bir_nzcv_expTheory
-      open bir_interval_expTheory
-      in [
-        type_of_bir_exp_def,
-        bir_var_type_def,
-        bir_type_is_Imm_def,
-        type_of_bir_imm_def,
-        BExp_Aligned_type_of,
-        BExp_unchanged_mem_interval_distinct_type_of,
-        bir_number_of_mem_splits_REWRS,
-        BType_Bool_def,
-        bir_exp_true_def,
-        bir_exp_false_def,
-        BExp_MSB_type_of,
-        BExp_nzcv_ADD_DEFS,
-        BExp_nzcv_SUB_DEFS,
-        n2bs_def,
-        BExp_word_bit_def,
-        BExp_Align_type_of,
-        BExp_ror_type_of,
-        BExp_LSB_type_of,
-        BExp_word_bit_exp_type_of,
-        BExp_ADD_WITH_CARRY_type_of,
-        BExp_word_reverse_type_of,
-        BExp_ror_exp_type_of
-      ] end;
-
-Theorem bprog_P_entails_thm[local]:
-  P_entails_an_interpret
-   (bir_symb_rec_sbir ^bprog_tm)
-   (P_bircont ^birenvtyl_tm ^bspec_pre_tm)
-   (birs_symb_to_symbst ^birs_state_init_pre_tm)
-Proof
-  ASSUME_TAC (GSYM prog_vars_thm) >>
-  `^prog_vars_tm = MAP PairToBVar ^birenvtyl_tm` by (
-    SIMP_TAC std_ss [birenvtyl_def, listTheory.MAP_MAP_o, PairToBVar_BVarToPair_I_thm, listTheory.MAP_ID]
-  ) >>
-  POP_ASSUM (fn thm => FULL_SIMP_TAC std_ss [thm]) >>
-  IMP_RES_TAC (SIMP_RULE std_ss [] P_bircont_entails_thm) >>
-
-  SIMP_TAC std_ss [] >>
-  POP_ASSUM (ASSUME_TAC o SPEC bspec_pre_tm) >>
-  `bir_vars_of_exp ^bspec_pre_tm SUBSET set (MAP PairToBVar ^birenvtyl_tm)` by EVAL_TAC >>
-  POP_ASSUM (fn thm => FULL_SIMP_TAC std_ss [thm]) >>
-  `ALL_DISTINCT (MAP FST ^birenvtyl_tm)` by EVAL_TAC >>
-  POP_ASSUM (fn thm => FULL_SIMP_TAC std_ss [thm]) >>
-  `IS_SOME (type_of_bir_exp ^bspec_pre_tm)` by (
-    SIMP_TAC std_ss [bspec_pre_def] >>
-    CONV_TAC (RAND_CONV (SIMP_CONV (srw_ss()) type_of_bir_exp_thms)) >>
-    SIMP_TAC (std_ss++holBACore_ss) [optionTheory.option_CLAUSES]
-  ) >>
-  POP_ASSUM (fn thm => FULL_SIMP_TAC std_ss [thm])
-QED
-
-(* ........................... *)
-(* ........................... *)
-(* ........................... *)
-
-(* ........................... *)
-(* proof for each end state individually: *)
-
-val sys1 = (snd o dest_eq o concl o REWRITE_CONV [bsysprecond_thm]) birs_state_init_pre_tm;
-val (Pi_func, Pi_set) = dest_comb Pi_f; (* Pi_func should be exactly ``IMAGE birs_symb_to_symbst`` *)
-val sys2s = pred_setSyntax.strip_set Pi_set;
-
-(*
-val sys2 = hd sys2s;
-*)
-val strongpostcond_goals = List.map (fn sys2 => ``
-    sys1 = ^sys1 ==>
-    sys2 = ^sys2 ==>
-    birs_symb_matchstate sys1 H' bs ==>
-    bir_eval_exp ^bspec_pre_tm bs.bst_environ = SOME bir_val_true ==>
-    birs_symb_matchstate sys2 H' bs' ==>
-    bir_eval_exp ^bspec_post_tm bs'.bst_environ = SOME bir_val_true
-  ``) sys2s;
-
-(*
-val goal = hd strongpostcond_goals;
-*)
-val strongpostcond_thms = List.map (fn goal =>
-  prove(``^goal``, birs_strongpostcond_impl_TAC)
-) strongpostcond_goals;
-
-(*
-val sys2 = hd sys2s;
-*)
-val Pi_thms = List.map (fn sys2 =>
-  prove(``
-    sys1 = ^sys1 ==>
-    sys2 = ^sys2 ==>
-    birs_symb_matchstate sys1 H bs ==>
-    P_bircont ^birenvtyl_tm ^bspec_pre_tm (birs_symb_to_concst bs) ==>
-    symb_interpr_ext H' H ==>
-    birs_symb_matchstate sys2 H' bs' ==>
-    Q_bircont ^birs_state_end_lbl_tm (set ^prog_vars_tm) ^bspec_post_tm
-     (birs_symb_to_concst bs) (birs_symb_to_concst bs')
-  ``,
-    REPEAT STRIP_TAC >>
-    Q_bircont_SOLVE3CONJS_TAC prog_vars_thm >>
-
-    `birs_symb_matchstate sys1 H' bs` by (
-      METIS_TAC [bir_symb_soundTheory.birs_symb_matchstate_interpr_ext_IMP_matchstate_thm]
-    ) >>
-    FULL_SIMP_TAC std_ss [P_bircont_thm] >>
-    METIS_TAC strongpostcond_thms
-  )
-) sys2s;
-
-(* ........................... *)
-
-(* Q is implied by sys and Pi *)
-Theorem bprog_Pi_overapprox_Q_thm[local]:
-  Pi_overapprox_Q
-   (bir_symb_rec_sbir ^bprog_tm)
-   (P_bircont ^birenvtyl_tm ^bspec_pre_tm)
-   (birs_symb_to_symbst ^birs_state_init_pre_tm) ^Pi_f
-   (Q_bircont ^birs_state_end_lbl_tm (set ^prog_vars_tm) ^bspec_post_tm)
-Proof
-  REWRITE_TAC [bir_prop_transferTheory.bir_Pi_overapprox_Q_thm, bsysprecond_thm] >>
-  REPEAT GEN_TAC >>
-
-  REWRITE_TAC [pred_setTheory.IMAGE_INSERT, pred_setTheory.IMAGE_EMPTY, pred_setTheory.IN_INSERT, pred_setTheory.NOT_IN_EMPTY] >>
-  REPEAT STRIP_TAC >> (
-    FULL_SIMP_TAC std_ss [] >>
-    METIS_TAC Pi_thms
-  )
-QED
-(* ........................... *)
-
-(* apply the theorem for property transfer *)
-val bprog_prop_holds_thm =
-  SIMP_RULE (std_ss++birs_state_ss)
-    [birs_state_init_pre_GEN_def, birs_symb_symbst_pc_thm] (
-  MATCH_MP
-    (MATCH_MP
-      (MATCH_MP
-         birs_prop_transfer_thm
-         bprog_P_entails_thm)
-      bprog_Pi_overapprox_Q_thm)
-    analysis_thm);
-
-(* ........................... *)
-(* ........................... *)
-(* ........................... *)
-
-Theorem bir_abstract_jgmt_rel_thm[local] =
-  (MATCH_MP
-    (MATCH_MP prop_holds_TO_abstract_jgmt_rel_thm analysis_L_NOTIN_thm)
-    (REWRITE_RULE [] bprog_prop_holds_thm));
-
-(* ........................... *)
-(* now manage the pre and postconditions into contract friendly "bir_exec_to_labels_triple_precond/postcond", need to change precondition to "bir_env_vars_are_initialised" for set of program variables *)
-
-(* ........................... *)
-(* ........................... *)
-(* ........................... *)
-
-Theorem abstract_jgmt_rel_thm[local]:
- abstract_jgmt_rel (bir_ts ^bprog_tm)
-  (BL_Address (Imm64 ^init_addr_tm)) {BL_Address (Imm64 ^end_addr_tm)}
-  (\st. bir_exec_to_labels_triple_precond st ^bspec_pre_tm ^bprog_tm)
-  (\st st'. bir_exec_to_labels_triple_postcond st'
-    (\l. if l = BL_Address (Imm64 ^end_addr_tm)
-         then ^bspec_post_tm
-         else bir_exp_false) ^bprog_tm)
-Proof
-  MATCH_MP_TAC (REWRITE_RULE
-   [boolTheory.AND_IMP_INTRO] abstract_jgmt_rel_bir_exec_to_labels_triple_thm) >>
-  SIMP_TAC std_ss [] >>
-  EXISTS_TAC birenvtyl_tm >>
-
-  CONJ_TAC >- (
-    (* bpre subset *)
-    REWRITE_TAC [bspec_pre_def] >>
-    SIMP_TAC (std_ss++pred_setLib.PRED_SET_ss) [GSYM prog_vars_thm, prog_vars_def] >>
-    SIMP_TAC (std_ss++pred_setLib.PRED_SET_ss++holBACore_ss) [listTheory.MEM, pred_setTheory.IN_INSERT] >>
-    EVAL_TAC
-  ) >>
-
-  CONJ_TAC >- (
-    (* bpost subset *)
-    REWRITE_TAC [bspec_post_def] >>
-    SIMP_TAC (std_ss++pred_setLib.PRED_SET_ss) [GSYM prog_vars_thm, prog_vars_def] >>
-    SIMP_TAC (std_ss++pred_setLib.PRED_SET_ss++holBACore_ss) [listTheory.MEM, pred_setTheory.IN_INSERT]
-  ) >>
-
-  CONJ_TAC >- (
-    (* bpost is bool *)
-    REWRITE_TAC [bspec_post_def] >>
-    SIMP_TAC (std_ss++holBACore_ss) [bir_is_bool_exp_REWRS, type_of_bir_exp_def]
-  ) >>
-
-  CONJ_TAC >- (
-    (* ALL_DISTINCT envtyl *)
-    SIMP_TAC (std_ss++listSimps.LIST_ss) [birenvtyl_EVAL_thm] >>
-    EVAL_TAC
-  ) >>
-
-  CONJ_TAC >- (
-    (* envtyl = vars_of_prog *)
-    REWRITE_TAC [GSYM prog_vars_thm] >>
-    SIMP_TAC std_ss [birenvtyl_def, listTheory.MAP_MAP_o, PairToBVar_BVarToPair_I_thm, listTheory.MAP_ID]
-  ) >>
-
-  METIS_TAC [bir_abstract_jgmt_rel_thm, prog_vars_thm]
-QED
-
-Theorem bspec_cont_thm[local]:
- bir_cont ^bprog_tm bir_exp_true
+Theorem bspec_cont_swap:
+ bir_cont bir_swap_prog bir_exp_true
   (BL_Address (Imm64 ^init_addr_tm)) {BL_Address (Imm64 ^end_addr_tm)} {}
   ^bspec_pre_tm
   (\l. if l = BL_Address (Imm64 ^end_addr_tm)
        then ^bspec_post_tm
        else bir_exp_false)
 Proof
- `{BL_Address (Imm64 ^end_addr_tm)} <> {}` by fs [] >>
- MP_TAC ((Q.SPECL [
-  `BL_Address (Imm64 ^init_addr_tm)`,
-  `{BL_Address (Imm64 ^end_addr_tm)}`,
-  `^bspec_pre_tm`,
-  `\l. if l = BL_Address (Imm64 ^end_addr_tm)
-       then ^bspec_post_tm
-       else bir_exp_false`
- ] o SPEC bprog_tm o INST_TYPE [Type.alpha |-> Type`:'observation_type`])
-  abstract_jgmt_rel_bir_cont) >>
- rw [] >>
- METIS_TAC [abstract_jgmt_rel_thm]
-QED
-
-Theorem bspec_cont_swap:
- bir_cont bir_swap_prog bir_exp_true
-  (BL_Address (Imm64 ^init_addr_tm)) {BL_Address (Imm64 ^end_addr_tm)} {}
-  (bspec_swap_pre pre_x10 pre_x11 pre_x10_mem_deref pre_x11_mem_deref)
-  (\l. if l = BL_Address (Imm64 ^end_addr_tm)
-       then bspec_swap_post pre_x10 pre_x11 pre_x10_mem_deref pre_x11_mem_deref
-       else bir_exp_false)
-Proof
- rw [bir_prog_def,bspec_cont_thm]
+ rw [bir_swap_prog_def,bspec_cont_thm]
 QED
 
 val _ = export_theory ();
